selectors automation: wip

ulib/experimental/Steel.SelEffect.fsti
@@ -7,8 +7,8 @@ open FStar.Ghost
 
 (* Normalization helpers *)
 
+irreducible let framing_implicit : unit = ()
 irreducible let __steel_reduce__ : unit = ()
-
 
 (* Definition of a selector for a given slprop *)
 
@@ -71,11 +71,15 @@ let rec sel_of (p:vprop) : selector (t_of p) (hp_of p) = match p with
      let sel2 = sel_of p2 in
      fun h -> (sel1 h, sel2 h)
 
+
+let return_pre (p:vprop) : vprop = p
+let return_post (#a:Type) (p:a -> vprop) : a -> vprop = p
+
 type pre_t = vprop
 type post_t (a:Type) = a -> vprop
 
-val can_be_split (p q:vprop) : prop
-val can_be_split_forall (#a:Type) (p q:post_t a) : prop
+val can_be_split (p q:vprop) : Type0
+let can_be_split_forall (#a:Type) (p q:post_t a) = forall x. can_be_split (p x) (q x)
 
 val can_be_split_trans (p q r:vprop)
 : Lemma
@@ -99,6 +103,19 @@ val can_be_split_refl (p:vprop)
 (* A restricted view of the heap,
    that only allows to access selectors of the current slprop *)
 
+let equiv_forall (#a:Type) (t1 t2:post_t a) : Type0
+  = t1 `can_be_split_forall` t2 /\ t2 `can_be_split_forall` t1
+
+val equiv_forall_split (#a:Type) (t1 t2:post_t a)
+  : Lemma (requires t1 `equiv_forall` t2)
+          (ensures can_be_split_forall t1 t2 /\ can_be_split_forall t2 t1)
+          [SMTPat (t1 `equiv_forall` t2)]
+
+let can_be_split_post (#a #b:Type) (t1:a -> post_t b) (t2:post_t b) =
+  forall (x:a). equiv_forall (t1 x) t2
+
+val equiv (p q:vprop) : prop
+
 let rmem (pre:vprop) =
   FExt.restricted_g_t
   (r0:vprop{can_be_split pre r0})
@@ -106,15 +123,16 @@ let rmem (pre:vprop) =
 
 (* Logical pre and postconditions can only access the restricted view of the heap *)
 
-type req_t (pre:pre_t) = rmem pre -> prop
+type req_t (pre:pre_t) = rmem pre -> Type0
 type ens_t (pre:pre_t) (a:Type) (post:post_t a) =
-  rmem pre -> (x:a) -> rmem (post x) -> prop
+  rmem pre -> (x:a) -> rmem (post x) -> Type0
 
 (* focus_rmem is an additional restriction of our view of memory.
    We expose it here to be able to reduce through normalization;
    Any valid application of focus_rmem h will be reduced to the application of h *)
 
 [@__steel_reduce__]
+unfold
 let unrestricted_focus_rmem (#r:vprop) (h:rmem r) (r0:vprop{r `can_be_split` r0})
   = fun (r':vprop{can_be_split r0 r'}) -> can_be_split_trans r r0 r'; h r'
 
@@ -123,124 +141,6 @@ let focus_rmem (#r: vprop) (h: rmem r) (r0: vprop{r `can_be_split` r0}) : Tot (r
  = FExt.on_dom_g
    (r':vprop{can_be_split r0 r'})
    (unrestricted_focus_rmem h r0)
-
-(* Defining the Steel effect with selectors *)
-
-val repr (a:Type) (pre:pre_t) (post:post_t a) (req:req_t pre) (ens:ens_t pre a post) : Type u#2
-
-unfold
-let return_req (p:vprop) : req_t p = fun _ -> True
-
-unfold
-let return_ens (#a:Type) (x:a) (p:a -> vprop) : ens_t (p x) a p = fun _ r _ -> r == x
-
-val return (a:Type u#a) (x:a) (p:a -> vprop)
-  : repr a (p x) p (return_req (p x)) (return_ens x p)
-
-unfold
-let bind_req (#a:Type) (#pre_f:vprop) (#post_f:a -> vprop)
-             (req_f:req_t pre_f) (ens_f:ens_t pre_f a post_f)
-             (req_g:(x:a -> req_t (post_f x)))
-  : req_t pre_f
-  = fun h -> req_f h /\ (forall (x:a) h1. ens_f h x h1 ==> req_g x h1)
-
-unfold
-let bind_ens (#a:Type) (#b:Type) (#pre_f:vprop) (#post_f:a -> vprop)
-             (req_f:req_t pre_f) (ens_f:ens_t pre_f a post_f)
-             (#post_g:b -> vprop) (ens_g:(x:a -> ens_t (post_f x) b post_g))
-  : ens_t pre_f b post_g
-  = fun h0 y h2 -> req_f h0 /\ (exists x h1. ens_f h0 x h1 /\ (ens_g x) h1 y h2)
-
-val bind (a:Type)
-         (b:Type)
-         (pre_f:vprop)
-         (post_f:a -> vprop)
-         (req_f:req_t pre_f)
-         (ens_f:ens_t pre_f a post_f)
-         (post_g:b -> vprop)
-         (req_g:(x:a -> req_t (post_f x)))
-         (ens_g:(x:a -> ens_t (post_f x) b post_g))
-         (f:repr a pre_f post_f req_f ens_f)
-         (g:(x:a -> repr b (post_f x) post_g (req_g x) (ens_g x)))
-   : repr b pre_f post_g
-          (bind_req req_f ens_f req_g)
-          (bind_ens req_f ens_f ens_g)
-
-unfold
-let subcomp_pre (#a:Type)
-                (#pre:vprop)
-                (#post:a -> vprop)
-                (req_f:req_t pre)
-                (ens_f:ens_t pre a post)
-                (req_g:req_t pre)
-                (ens_g:ens_t pre a post)
-   : pure_pre
-   = (forall h. req_g h ==> req_f h) /\
-     (forall h0 x h1. (req_g h0 /\ ens_f h0 x h1) ==> ens_g h0 x h1)
-
-val subcomp (a:Type)
-            (pre:vprop)
-            (post:a -> vprop)
-            (req_f:req_t pre)
-            (ens_f:ens_t pre a post)
-            (req_g:req_t pre)
-            (ens_g:ens_t pre a post)
-            (f:repr a pre post req_f ens_f)
-  : Pure (repr a pre post req_g ens_g)
-         (requires subcomp_pre req_f ens_f req_g ens_g)
-         (ensures fun _ -> True)
-
-[@@ allow_informative_binders]
-reifiable reflectable
-layered_effect {
-  SteelSel : a:Type
-        -> pre:pre_t
-        -> post:post_t a
-        -> req:req_t pre
-        -> ens:ens_t pre a post
-        -> Effect
-  with
-  repr = repr;
-  return = return;
-  bind = bind;
-  subcomp = subcomp
-}
-
-(* Defining a bind with pure functions *)
-
-unfold
-let bind_pure_steel_req (#a:Type)
-                        (wp:pure_wp a)
-                        (#pre_g:vprop)
-                        (req_g:a -> req_t pre_g)
-  : req_t pre_g
-  = FStar.Monotonic.Pure.wp_monotonic_pure ();
-    fun h -> wp (fun x -> req_g x h) /\ wp (fun _ -> True)
-
-unfold
-let bind_pure_steel_ens (#a:Type)
-                        (#b:Type)
-                        (wp:pure_wp a)
-                        (#pre_g:vprop)
-                        (#post_g:b -> vprop)
-                        (ens_g:a -> ens_t pre_g b post_g)
-   : ens_t pre_g b post_g
-   = fun h0 r h1 -> wp (fun _ -> True) /\ (exists x. (~ (wp (fun r -> r =!= x))) /\ ens_g x h0 r h1)
-
-val bind_pure_steel (a:Type)
-                    (b:Type)
-                    (wp:pure_wp a)
-                    (pre_g:vprop)
-                    (post_g:b -> vprop)
-                    (req_g:a -> req_t pre_g)
-                    (ens_g:a -> ens_t pre_g b post_g)
-                    (f:eqtype_as_type unit -> PURE a wp)
-                    (g:(x:a -> repr b pre_g post_g (req_g x) (ens_g x)))
-  : repr b pre_g post_g
-         (bind_pure_steel_req wp req_g)
-         (bind_pure_steel_ens wp ens_g)
-
-polymonadic_bind (PURE, SteelSel) |> SteelSel = bind_pure_steel
 
 (* State that all "atomic" subresources have the same selectors on both views *)
 
@@ -264,6 +164,324 @@ let rec frame_equalities
 
         frame_equalities p1 h01 h11 /\
         frame_equalities p2 h02 h12
+
+
+(* Defining the Steel effect with selectors *)
+
+val repr (a:Type) (pre:pre_t) (post:post_t a) (req:req_t pre) (ens:ens_t pre a post) : Type u#2
+
+unfold
+let return_req (p:vprop) : req_t p = fun _ -> True
+
+unfold
+let return_ens (a:Type) (x:a) (p:a -> vprop) : ens_t (p x) a p = fun _ r _ -> r == x
+
+(*
+ * Return is parametric in post (cf. return-scoping.txt)
+ *)
+val return (a:Type) (x:a) (#[@@ framing_implicit] p:a -> vprop)
+: repr a (return_pre (p x)) (return_post p) (return_req (p x)) (return_ens a x p)
+
+unfold
+let bind_req (#a:Type)
+  (#pre_f:pre_t) (#post_f:post_t a)
+  (req_f:req_t pre_f) (ens_f:ens_t pre_f a post_f)
+  (#pre_g:a -> pre_t)
+  (req_g:(x:a -> req_t (pre_g x)))
+  (_:squash (can_be_split_forall post_f pre_g))
+: req_t pre_f
+= fun m0 ->
+  req_f m0 /\
+  (forall (x:a) (m1:rmem (post_f x)). ens_f m0 x m1 ==> (req_g x) (focus_rmem m1 (pre_g x)))
+
+unfold
+let bind_ens (#a:Type) (#b:Type)
+  (#pre_f:pre_t) (#post_f:post_t a)
+  (req_f:req_t pre_f) (ens_f:ens_t pre_f a post_f)
+  (#pre_g:a -> pre_t) (#post_g:a -> post_t b)
+  (ens_g:(x:a -> ens_t (pre_g x) b (post_g x)))
+  (post:post_t b)
+  (_:squash (can_be_split_forall post_f pre_g))
+  (_:squash (can_be_split_post post_g post))
+: ens_t pre_f b post
+= fun m0 y m2 ->
+  req_f m0 /\
+  (exists (x:a) (m1:rmem (post_f x)). ens_f m0 x m1 /\ (ens_g x) (focus_rmem m1 (pre_g x)) y (focus_rmem m2 (post_g x y)))
+
+val bind (a:Type) (b:Type)
+  (#[@@ framing_implicit] pre_f:pre_t) (#[@@ framing_implicit] post_f:post_t a)
+  (#[@@ framing_implicit] req_f:req_t pre_f) (#[@@ framing_implicit] ens_f:ens_t pre_f a post_f)
+  (#[@@ framing_implicit] pre_g:a -> pre_t) (#[@@ framing_implicit] post_g:a -> post_t b)
+  (#[@@ framing_implicit] req_g:(x:a -> req_t (pre_g x))) (#[@@ framing_implicit] ens_g:(x:a -> ens_t (pre_g x) b (post_g x)))
+  (#[@@ framing_implicit] post:post_t b)
+  (#[@@ framing_implicit] p1:squash (can_be_split_forall post_f pre_g))
+  (#[@@ framing_implicit] p2:squash (can_be_split_post post_g post))
+  (f:repr a pre_f post_f req_f ens_f)
+  (g:(x:a -> repr b (pre_g x) (post_g x) (req_g x) (ens_g x)))
+: repr b
+    pre_f
+    post
+    (bind_req req_f ens_f req_g p1)
+    (bind_ens req_f ens_f ens_g post p1 p2)
+
+unfold
+let subcomp_pre (#a:Type)
+  (#pre_f:pre_t) (#post_f:post_t a) (req_f:req_t pre_f) (ens_f:ens_t pre_f a post_f)
+  (#pre_g:pre_t) (#post_g:post_t a) (req_g:req_t pre_g) (ens_g:ens_t pre_g a post_g)
+  (_:squash (can_be_split pre_g pre_f))
+  (_:squash (can_be_split_forall post_f post_g))
+: pure_pre
+= (forall (m0:rmem pre_g). req_g m0 ==> req_f (focus_rmem m0 pre_f)) /\
+  (forall (m0:rmem pre_g) (x:a) (m1:rmem (post_f x)). ens_f (focus_rmem m0 pre_f) x m1 ==> ens_g m0 x (focus_rmem m1 (post_g x)))
+
+val subcomp (a:Type)
+  (#[@@ framing_implicit] pre_f:pre_t) (#[@@ framing_implicit] post_f:post_t a)
+  (#[@@ framing_implicit] req_f:req_t pre_f) (#[@@ framing_implicit] ens_f:ens_t pre_f a post_f)
+  (#[@@ framing_implicit] pre_g:pre_t) (#[@@ framing_implicit] post_g:post_t a)
+  (#[@@ framing_implicit] req_g:req_t pre_g) (#[@@ framing_implicit] ens_g:ens_t pre_g a post_g)
+  (#[@@ framing_implicit] p1:squash (can_be_split pre_g pre_f))
+  (#[@@ framing_implicit] p2:squash (can_be_split_forall post_f post_g))
+  (f:repr a pre_f post_f req_f ens_f)
+: Pure (repr a pre_g post_g req_g ens_g)
+  (requires subcomp_pre #a #pre_f #post_f req_f ens_f req_g ens_g p1 p2)
+  (ensures fun _ -> True)
+
+[@@allow_informative_binders]
+reifiable reflectable
+layered_effect {
+  SteelSelF: a:Type -> pre:pre_t -> post:post_t a -> req_t pre -> ens_t pre a post -> Effect
+  with repr = repr;
+       return = return;
+       bind = bind;
+       subcomp = subcomp
+}
+
+[@@allow_informative_binders]
+reifiable reflectable
+new_effect SteelSel = SteelSelF
+
+
+(*
+ * Onto polymonadic binds
+ *)
+
+(*
+ * First the bind between two unframed computations
+ *
+ * Add a frame to each
+ *)
+
+unfold
+let bind_steel_steel_req (#a:Type)
+  (#pre_f:pre_t) (#post_f:post_t a)
+  (req_f:req_t pre_f) (ens_f:ens_t pre_f a post_f)
+  (#pre_g:a -> pre_t)
+  (req_g:(x:a -> req_t (pre_g x)))
+  (frame_f:vprop) (frame_g:a -> vprop)
+  (_:squash (can_be_split_forall (fun x -> post_f x `star` frame_f) (fun x -> pre_g x `star` frame_g x)))
+: req_t (pre_f `star` frame_f)
+= fun m0 ->
+  // TODO: Add frame in "precondition" of req_g
+  req_f (focus_rmem m0 pre_f) /\
+  (forall (x:a) (m1:rmem (post_f x `star` frame_f)). (
+    can_be_split_trans (post_f x `star` frame_f) (pre_g x `star` frame_g x) (pre_g x);
+    ens_f (focus_rmem m0 pre_f) x (focus_rmem m1 (post_f x)) ==>
+      (req_g x) (focus_rmem m1 (pre_g x))))
+
+unfold
+let bind_steel_steel_ens (#a:Type) (#b:Type)
+  (#pre_f:pre_t) (#post_f:post_t a)
+  (req_f:req_t pre_f) (ens_f:ens_t pre_f a post_f)
+  (#pre_g:a -> pre_t) (#post_g:a -> post_t b)
+  (ens_g:(x:a -> ens_t (pre_g x) b (post_g x)))
+  (frame_f:vprop) (frame_g:a -> vprop)
+  (post:post_t b)
+  (_:squash (can_be_split_forall (fun x -> post_f x `star` frame_f) (fun x -> pre_g x `star` frame_g x)))
+  (_:squash (can_be_split_post (fun x y -> post_g x y `star` frame_g x) post))
+: ens_t (pre_f `star` frame_f) b post
+= fun m0 y m2 ->
+  // TODO: Add frames
+  req_f (focus_rmem m0 pre_f) /\
+  (exists (x:a) (m1:rmem (post_f x `star` frame_f)). (
+    can_be_split_trans (post_f x `star` frame_f) (pre_g x `star` frame_g x) (pre_g x);
+    can_be_split_trans (post y) (post_g x y `star` frame_g x) (post_g x y);
+    ens_f (focus_rmem m0 pre_f) x (focus_rmem m1 (post_f x)) /\
+    (ens_g x) (focus_rmem m1 (pre_g x)) y (focus_rmem m2 (post_g x y))))
+
+val bind_steel_steel (a:Type) (b:Type)
+  (#[@@ framing_implicit] pre_f:pre_t) (#[@@ framing_implicit] post_f:post_t a)
+  (#[@@ framing_implicit] req_f:req_t pre_f) (#[@@ framing_implicit] ens_f:ens_t pre_f a post_f)
+  (#[@@ framing_implicit] pre_g:a -> pre_t) (#[@@ framing_implicit] post_g:a -> post_t b)
+  (#[@@ framing_implicit] req_g:(x:a -> req_t (pre_g x))) (#[@@ framing_implicit] ens_g:(x:a -> ens_t (pre_g x) b (post_g x)))
+  (#[@@ framing_implicit] frame_f:vprop) (#[@@ framing_implicit] frame_g:a -> vprop)
+  (#[@@ framing_implicit] post:post_t b)
+  (#[@@ framing_implicit] p:squash (can_be_split_forall
+    (fun x -> post_f x `star` frame_f) (fun x -> pre_g x `star` frame_g x)))
+  (#[@@ framing_implicit] p2:squash (can_be_split_post (fun x y -> post_g x y `star` frame_g x) post))
+  (f:repr a pre_f post_f req_f ens_f)
+  (g:(x:a -> repr b (pre_g x) (post_g x) (req_g x) (ens_g x)))
+: repr b
+    (pre_f `star` frame_f)
+    post
+    (bind_steel_steel_req req_f ens_f req_g frame_f frame_g p)
+    (bind_steel_steel_ens req_f ens_f ens_g frame_f frame_g post p p2)
+
+(*
+ * Note that the output is a framed computation, hence SteelF
+ *)
+
+polymonadic_bind (SteelSel, SteelSel) |> SteelSelF = bind_steel_steel
+
+
+(*
+ * Steel, SteelF: frame the first computation
+ *)
+
+unfold
+let bind_steel_steelf_req (#a:Type)
+  (#pre_f:pre_t) (#post_f:post_t a)
+  (req_f:req_t pre_f) (ens_f:ens_t pre_f a post_f)
+  (#pre_g:a -> pre_t)
+  (req_g:(x:a -> req_t (pre_g x)))
+  (frame_f:vprop)
+  (_:squash (can_be_split_forall (fun x -> post_f x `star` frame_f) pre_g))
+: req_t (pre_f `star` frame_f)
+= fun m0 ->
+  // TODO: Add frame propagation in precondition of req_g
+  req_f (focus_rmem m0 pre_f) /\
+  (forall (x:a) (m1:rmem (post_f x `star` frame_f)). ens_f (focus_rmem m0 pre_f) x (focus_rmem m1 (post_f x)) ==> (req_g x) (focus_rmem m1 (pre_g x)))
+
+unfold
+let bind_steel_steelf_ens (#a:Type) (#b:Type)
+  (#pre_f:pre_t) (#post_f:post_t a)
+  (req_f:req_t pre_f) (ens_f:ens_t pre_f a post_f)
+  (#pre_g:a -> pre_t) (#post_g:a -> post_t b)
+  (ens_g:(x:a -> ens_t (pre_g x) b (post_g x)))
+  (frame_f:vprop)
+  (post:post_t b)
+  (_:squash (can_be_split_forall (fun x -> post_f x `star` frame_f) pre_g))
+  (_: squash (can_be_split_post post_g post))
+: ens_t (pre_f `star` frame_f) b post
+= fun m0 y m2 ->
+  // TODO: Add frame propagation
+  req_f (focus_rmem m0 pre_f) /\
+  (exists (x:a) (m1:rmem (post_f x `star` frame_f)). ens_f (focus_rmem m0 pre_f) x (focus_rmem m1 (post_f x)) /\ (ens_g x) (focus_rmem m1 (pre_g x)) y (focus_rmem m2 (post_g x y)))
+
+val bind_steel_steelf (a:Type) (b:Type)
+  (#[@@ framing_implicit] pre_f:pre_t) (#[@@ framing_implicit] post_f:post_t a)
+  (#[@@ framing_implicit] req_f:req_t pre_f) (#[@@ framing_implicit] ens_f:ens_t pre_f a post_f)
+  (#[@@ framing_implicit] pre_g:a -> pre_t) (#[@@ framing_implicit] post_g:a -> post_t b)
+  (#[@@ framing_implicit] req_g:(x:a -> req_t (pre_g x))) (#[@@ framing_implicit] ens_g:(x:a -> ens_t (pre_g x) b (post_g x)))
+  (#[@@ framing_implicit] frame_f:vprop)
+  (#[@@ framing_implicit] post:post_t b)
+  (#[@@ framing_implicit] p:squash (can_be_split_forall (fun x -> post_f x `star` frame_f) pre_g))
+  (#[@@ framing_implicit] p2: squash (can_be_split_post post_g post))
+  (f:repr a pre_f post_f req_f ens_f)
+  (g:(x:a -> repr b (pre_g x) (post_g x) (req_g x) (ens_g x)))
+: repr b
+    (pre_f `star` frame_f)
+    post
+    (bind_steel_steelf_req req_f ens_f req_g frame_f p)
+    (bind_steel_steelf_ens req_f ens_f ens_g frame_f post p p2)
+
+polymonadic_bind (SteelSel, SteelSelF) |> SteelSelF = bind_steel_steelf
+
+
+(*
+ * SteelF, Steel: frame the second computation
+ *)
+
+unfold
+let bind_steelf_steel_req (#a:Type)
+  (#pre_f:pre_t) (#post_f:post_t a)
+  (req_f:req_t pre_f) (ens_f:ens_t pre_f a post_f)
+  (#pre_g:a -> pre_t)
+  (req_g:(x:a -> req_t (pre_g x)))
+  (frame_g:a -> vprop)
+  (_:squash (can_be_split_forall post_f (fun x -> pre_g x `star` frame_g x)))
+: req_t pre_f
+= fun m0 ->
+  req_f m0 /\
+  (forall (x:a) (m1:rmem (post_f x)). (
+    can_be_split_trans (post_f x) (pre_g x `star` frame_g x) (pre_g x);
+    ens_f m0 x m1 ==> (req_g x) (focus_rmem m1 (pre_g x))))
+
+unfold
+let bind_steelf_steel_ens (#a:Type) (#b:Type)
+  (#pre_f:pre_t) (#post_f:post_t a)
+  (req_f:req_t pre_f) (ens_f:ens_t pre_f a post_f)
+  (#pre_g:a -> pre_t) (#post_g:a -> post_t b)
+  (ens_g:(x:a -> ens_t (pre_g x) b (post_g x)))
+  (frame_g:a -> vprop)
+  (post:post_t b)
+  (_:squash (can_be_split_forall post_f (fun x -> pre_g x `star` frame_g x)))
+  (_:squash (can_be_split_post (fun x y -> post_g x y `star` frame_g x) post))
+: ens_t pre_f b post
+= fun m0 y m2 ->
+  req_f m0 /\
+  (exists (x:a) (m1:rmem (post_f x)). (
+    can_be_split_trans (post_f x) (pre_g x `star` frame_g x) (pre_g x);
+    can_be_split_trans (post y) (post_g x y `star` frame_g x) (post_g x y);
+    ens_f m0 x m1 /\ (ens_g x) (focus_rmem m1 (pre_g x)) y (focus_rmem m2 (post_g x y))))
+
+val bind_steelf_steel (a:Type) (b:Type)
+  (#[@@ framing_implicit] pre_f:pre_t) (#[@@ framing_implicit] post_f:post_t a)
+  (#[@@ framing_implicit] req_f:req_t pre_f) (#[@@ framing_implicit] ens_f:ens_t pre_f a post_f)
+  (#[@@ framing_implicit] pre_g:a -> pre_t) (#[@@ framing_implicit] post_g:a -> post_t b)
+  (#[@@ framing_implicit] req_g:(x:a -> req_t (pre_g x))) (#[@@ framing_implicit] ens_g:(x:a -> ens_t (pre_g x) b (post_g x)))
+  (#[@@ framing_implicit] frame_g:a -> vprop)
+  (#[@@ framing_implicit] post:post_t b)
+  (#[@@ framing_implicit] p:squash (can_be_split_forall post_f (fun x -> pre_g x `star` frame_g x)))
+  (#[@@ framing_implicit] p2:squash (can_be_split_post (fun x y -> post_g x y `star` frame_g x) post))
+  (f:repr a pre_f post_f req_f ens_f)
+  (g:(x:a -> repr b (pre_g x) (post_g x) (req_g x) (ens_g x)))
+: repr b
+    pre_f
+    post
+    (bind_steelf_steel_req req_f ens_f req_g frame_g p)
+    (bind_steelf_steel_ens req_f ens_f ens_g frame_g post p p2)
+
+
+polymonadic_bind (SteelSelF, SteelSel) |> SteelSelF = bind_steelf_steel
+
+(*
+//  * PURE, Steel(F) bind
+//  *)
+
+unfold
+let bind_pure_steel__req (#a:Type) (wp:pure_wp a)
+  (#pre:pre_t) (req:a -> req_t pre)
+: req_t pre
+= fun m -> wp (fun x -> (req x) m) /\ as_requires wp
+
+unfold
+let bind_pure_steel__ens (#a:Type) (#b:Type)
+  (wp:pure_wp a)
+  (#pre:pre_t) (#post:post_t b) (ens:a -> ens_t pre b post)
+: ens_t pre b post
+= fun m0 r m1 -> as_requires wp /\ (exists (x:a). as_ensures wp x /\ (ens x) m0 r m1)
+
+val bind_pure_steel_ (a:Type) (b:Type)
+  (wp:pure_wp a)
+  (#[@@ framing_implicit] pre:pre_t) (#[@@ framing_implicit] post:post_t b)
+  (#[@@ framing_implicit] req:a -> req_t pre) (#[@@ framing_implicit] ens:a -> ens_t pre b post)
+  (f:eqtype_as_type unit -> PURE a wp) (g:(x:a -> repr b pre post (req x) (ens x)))
+: repr b
+    pre
+    post
+    (bind_pure_steel__req wp req)
+    (bind_pure_steel__ens wp ens)
+
+polymonadic_bind (PURE, SteelSel) |> SteelSel = bind_pure_steel_
+polymonadic_bind (PURE, SteelSelF) |> SteelSelF = bind_pure_steel_
+
+(*
+//  * subcomp relation from SteelF to Steel
+//  *)
+
+polymonadic_subcomp SteelSelF <: SteelSel = subcomp
+
+
 
 (* Some helper functions *)
 
@@ -350,6 +568,1124 @@ let sel (#a:Type) (#p:vprop) (h:rmem p) (r:ref a)
   : Ghost a (requires can_be_split p (vptr r)) (ensures fun _ -> True)
   = h (vptr r)
 
+
+(* Framing Tactic *)
+
+val equiv_can_be_split (p1 p2:vprop) : Lemma
+  (requires p1 `equiv` p2)
+  (ensures p1 `can_be_split` p2)
+
+
+open FStar.Tactics
+
+open FStar.Tactics.CanonCommMonoidSimple.Equiv
+
+val equiv_refl (x:vprop) : Lemma (equiv x x)
+
+val equiv_sym (x y:vprop) : Lemma
+  (requires equiv x y)
+  (ensures equiv y x)
+
+val equiv_trans (x y z:vprop) : Lemma
+  (requires equiv x y /\ equiv y z)
+  (ensures equiv x z)
+
+module CE = FStar.Algebra.CommMonoid.Equiv
+
+inline_for_extraction noextract let req : CE.equiv vprop =
+  CE.EQ equiv
+     equiv_refl
+     equiv_sym
+     equiv_trans
+
+val cm_identity (x:vprop) : Lemma ((vemp `star` x) `equiv` x)
+
+val star_commutative (p1 p2:vprop)
+  : Lemma ((p1 `star` p2) `equiv` (p2 `star` p1))
+
+val star_associative (p1 p2 p3:vprop)
+  : Lemma (((p1 `star` p2) `star` p3)
+           `equiv`
+           (p1 `star` (p2 `star` p3)))
+
+val star_congruence (p1 p2 p3 p4:vprop)
+  : Lemma (requires p1 `equiv` p3 /\ p2 `equiv` p4)
+          (ensures (p1 `star` p2) `equiv` (p3 `star` p4))
+
+
+inline_for_extraction noextract let rm : CE.cm vprop req =
+  CE.CM vemp
+     star
+     cm_identity
+     star_associative
+     star_commutative
+     star_congruence
+
+exception Appears
+
+(** Decides whether a top-level name [nm] syntactically
+// appears in the term [t]. *)
+let name_appears_in (nm:name) (t:term) : Tac bool =
+  // let ff (t:term) : Tac term = raise Appears in
+  let ff (t : term) : Tac term =
+    match t with
+    | Tv_FVar fv ->
+        let uh = inspect_fv fv in
+        let nm1 = implode_qn nm in
+        let nm2 = implode_qn uh in
+        dump (nm1 ^ " " ^ nm2);
+        if nm1 = nm2 then (
+          dump "compared";
+        raise Appears)
+        else dump "not compared";
+      t
+    | t -> t
+  in
+  try ignore (visit_tm ff t); false with
+  | Appears -> true
+  | e -> dump "pre raise"; raise e
+
+
+let term_appears_in (t:term) (i:term) : Tac bool = let b = name_appears_in (explode_qn (term_to_string t)) i in
+  dump "after";
+  b
+
+
+
+let atom : eqtype = int
+
+let rec atoms_to_string (l:list atom) = match l with
+  | [] -> ""
+  | hd::tl -> string_of_int hd ^ " " ^ atoms_to_string tl
+
+type exp : Type =
+  | Unit : exp
+  | Mult : exp -> exp -> exp
+  | Atom : atom -> exp
+
+let amap (a:Type) = list (atom * a) * a
+let const (#a:Type) (xa:a) : amap a = ([], xa)
+let select (#a:Type) (x:atom) (am:amap a) : Tot a =
+  match List.Tot.Base.assoc #atom #a x (fst am) with
+  | Some a -> a
+  | _ -> snd am
+let update (#a:Type) (x:atom) (xa:a) (am:amap a) : amap a =
+  (x, xa)::fst am, snd am
+
+let is_uvar (t:term) : Tac bool = match t with
+  | Tv_Uvar _ _ -> true
+  | Tv_App _ _ ->
+      let hd, args = collect_app t in
+      Tv_Uvar? hd
+  | _ -> false
+
+(* For a given term t, collect all terms in the list l with the same head symbol *)
+let rec get_candidates (t:term) (l:list term) : Tac (list term) =
+  let name, _ = collect_app t in
+  match l with
+  | [] -> []
+  | hd::tl ->
+      let n, _ = collect_app hd in
+      if term_eq n name then (
+        hd::(get_candidates t tl)
+      ) else get_candidates t tl
+
+(* Try to remove a term that is exactly matching, not just that can be unified *)
+let rec trivial_cancel (t:atom) (l:list atom) =
+  match l with
+  | [] -> false, l
+  | hd::tl ->
+      if hd = t then
+        // These elements match, we remove them
+        true, tl
+      else (let b, res = trivial_cancel t tl in b, hd::res)
+
+(* Call trivial_cancel on all elements of l1.
+   The first two lists returned are the remainders of l1 and l2.
+   The last two lists are the removed parts of l1 and l2, with
+   the additional invariant that they are equal *)
+let rec trivial_cancels (l1 l2:list atom) (am:amap term)
+  : Tac (list atom * list atom * list atom * list atom) =
+  match l1 with
+  | [] -> [], l2, [], []
+  | hd::tl ->
+      let b, l2'   = trivial_cancel hd l2 in
+      let l1', l2', l1_del, l2_del = trivial_cancels tl l2' am in
+      (if b then l1' else hd::l1'), l2',
+      (if b then hd::l1_del else l1_del), (if b then hd::l2_del else l2_del)
+
+exception Failed
+exception Success
+
+(* For a list of candidates l, count the number that can unify with t.
+   Does not try to unify with a uvar, this will be done at the very end.
+   Tries to unify with slprops with a different head symbol, it might
+   be an abbreviation
+ *)
+let rec try_candidates (t:atom) (l:list atom) (am:amap term) : Tac (atom * int) =
+  match l with
+  | [] -> t, 0
+  | hd::tl ->
+      if is_uvar (select hd am) then (try_candidates t tl am)
+      else
+        // Encapsulate unify in a try/with to ensure unification is not actually performed
+        let res = try if unify (select t am) (select hd am) then raise Success else raise Failed
+                  with | Success -> true | _ -> false in
+        let t', n' = try_candidates t tl am in
+        if res then hd, 1 + n'  else t', n'
+
+(* Remove the given term from the list. Only to be called when
+   try_candidates succeeded *)
+let rec remove_from_list (t:atom) (l:list atom) : Tac (list atom) =
+  match l with
+  | [] -> fail "atom in remove_from_list not found: should not happen"; []
+  | hd::tl -> if t = hd then tl else hd::remove_from_list t tl
+
+(* Check if two lists of slprops are equivalent by recursively calling
+   try_candidates.
+   Assumes that only l2 contains terms with the head symbol unresolved.
+   It returns all elements that were not resolved during this iteration *)
+let rec equivalent_lists_once (l1 l2 l1_del l2_del:list atom) (am:amap term)
+  : Tac (list atom * list atom * list atom * list atom) =
+  match l1 with
+  | [] -> [], l2, l1_del, l2_del
+  | hd::tl ->
+    let t, n = try_candidates hd l2 am in
+    // if n = 0 then
+    //   fail ("not equiv: no candidate found for scrutinee " ^ term_to_string (select hd am))
+    if n = 1 then (
+      let l2 = remove_from_list t l2 in
+      equivalent_lists_once tl l2 (hd::l1_del) (t::l2_del) am
+    ) else
+      // Either too many candidates for this scrutinee, or no candidate but the uvar
+      let rem1, rem2, l1'_del, l2'_del = equivalent_lists_once tl l2 l1_del l2_del am in
+      hd::rem1, rem2, l1'_del, l2'_del
+
+let get_head (l:list atom) (am:amap term) : term = match l with
+  | [] -> `()
+  | hd::_ -> select hd am
+
+let is_only_uvar (l:list atom) (am:amap term) : Tac bool =
+  if List.Tot.Base.length l = 1 then is_uvar (select (List.Tot.Base.hd l) am)
+  else false
+
+(* Assumes that u is a uvar, checks that all variables in l can be unified with it.
+   Later in the tactic, the uvar will be unified to a star of l *)
+let rec try_unifying_remaining (l:list atom) (u:term) (am:amap term) : Tac unit =
+  match l with
+  | [] -> ()
+  | hd::tl ->
+      try if unify u (select hd am) then raise Success else raise Failed with
+      | Success -> try_unifying_remaining tl u am
+      | _ -> fail ("could not find candidate for scrutinee " ^ term_to_string (select hd am))
+
+(* Recursively calls equivalent_lists_once.
+   Stops when we're done with unification, or when we didn't make any progress
+   If we didn't make any progress, we have too many candidates for some terms.
+   Accumulates rewritings of l1 and l2 in l1_del and l2_del, with the invariant
+   that the two lists are unifiable at any point
+   The boolean indicates if there is a leftover empty frame
+   *)
+let rec equivalent_lists' (n:nat) (l1 l2 l1_del l2_del:list atom) (am:amap term)
+  : Tac (list atom * list atom * bool) =
+  match l1 with
+  | [] -> begin match l2 with
+    | [] -> (l1_del, l2_del, false)
+    | [hd] ->
+      // Succeed if there is only one uvar left in l2, which can be therefore
+      // be unified with emp
+      if is_uvar (select hd am) then (
+        // xsdenote is left associative: We put hd at the top to get
+        // ?u `star` p <==> emp `star` p
+        (l1_del, hd :: l2_del, true))
+      else fail ("could not find candidates for " ^ term_to_string (get_head l2 am))
+    | _ -> fail ("could not find candidates for " ^ term_to_string (get_head l2 am))
+    end
+  | _ ->
+    if is_only_uvar l2 am then (
+      // Terms left in l1, but only a uvar left in l2.
+      // Put all terms left at the end of l1_rem, so that they can be unified
+      // with exactly the uvar because of the structure of xsdenote
+      try_unifying_remaining l1 (get_head l2 am) am;
+      l1_del @ l1, l2_del @ l2, false
+    ) else
+      let rem1, rem2, l1_del', l2_del' = equivalent_lists_once l1 l2 l1_del l2_del am in
+      let n' = List.Tot.length rem1 in
+      if n' >= n then
+        // Should always be smaller or equal to n
+        // If it is equal, no progress was made.
+        fail ("could not find candidate for scrutinee " ^ term_to_string (get_head rem2 am))
+      else equivalent_lists' n' rem1 rem2 l1_del' l2_del' am
+
+(* Checks if term for atom t unifies with fall uvars in l *)
+let rec unifies_with_all_uvars (t:term) (l:list atom) (am:amap term) : Tac bool =
+  match l with
+  | [] -> true
+  | hd::tl ->
+      if unifies_with_all_uvars t tl am then (
+        // Unified with tail, try this term
+        let hd_t = select hd am in
+        if is_uvar hd_t then (
+          // The head term is a uvar, try unifying
+          try if unify t hd_t then raise Success else raise Failed
+          with | Success -> true | _ -> false
+        ) else true // The uvar is not a head term, we do not need to try it
+      ) else false
+
+(* Puts all terms in l1 that cannot unify with the uvars in l2 at the top:
+   They need to be solved first *)
+let rec most_restricted_at_top (l1 l2:list atom) (am:amap term) : Tac (list atom) =
+  match l1 with
+  | [] -> []
+  | hd::tl ->
+    if unifies_with_all_uvars (select hd am) l2 am then (most_restricted_at_top tl l2 am)@[hd]
+    else hd::(most_restricted_at_top tl l2 am)
+
+(* First remove all trivially equal terms, then try to decide equivalence.
+   Assumes that l1 does not contain any slprop uvar.
+   If it succeeds, returns permutations of l1, l2, and a boolean indicating
+   if l2 has a trailing empty frame to be unified
+*)
+let equivalent_lists (l1 l2:list atom) (am:amap term) : Tac (list atom * list atom * bool) =
+  let l1, l2, l1_del, l2_del = trivial_cancels l1 l2 am in
+  let l1 = most_restricted_at_top l1 l2 am in
+  let n = List.Tot.length l1 in
+  let l1_del, l2_del, emp_frame = equivalent_lists' n l1 l2 l1_del l2_del am in
+  l1_del, l2_del, emp_frame
+
+open FStar.Reflection.Derived.Lemmas
+
+let rec list_to_string (l:list term) : Tac string =
+  match l with
+  | [] -> "end"
+  | hd::tl -> term_to_string hd ^ " " ^ list_to_string tl
+
+open FStar.Algebra.CommMonoid.Equiv
+
+let rec mdenote (#a:Type u#aa) (eq:equiv a) (m:cm a eq) (am:amap a) (e:exp) : a =
+  match e with
+  | Unit -> CM?.unit m
+  | Atom x -> select x am
+  | Mult e1 e2 -> CM?.mult m (mdenote eq m am e1) (mdenote eq m am e2)
+
+let rec xsdenote (#a:Type) (eq:equiv a) (m:cm a eq) (am:amap a) (xs:list atom) : a =
+  match xs with
+  | [] -> CM?.unit m
+  | [x] -> select x am
+  | x::xs' -> CM?.mult m (select x am) (xsdenote eq m am xs')
+
+let rec flatten (e:exp) : list atom =
+  match e with
+  | Unit -> []
+  | Atom x -> [x]
+  | Mult e1 e2 -> flatten e1 @ flatten e2
+
+let rec flatten_correct_aux (#a:Type) (eq:equiv a) (m:cm a eq) (am:amap a) (xs1 xs2:list atom)
+  : Lemma (xsdenote eq m am (xs1 @ xs2) `EQ?.eq eq` CM?.mult m (xsdenote eq m am xs1)
+                                                               (xsdenote eq m am xs2)) =
+  match xs1 with
+  | [] ->
+      CM?.identity m (xsdenote eq m am xs2);
+      EQ?.symmetry eq (CM?.mult m (CM?.unit m) (xsdenote eq m am xs2)) (xsdenote eq m am xs2)
+  | [x] -> (
+      if (Nil? xs2)
+      then (right_identity eq m (select x am);
+            EQ?.symmetry eq (CM?.mult m (select x am) (CM?.unit m)) (select x am))
+      else EQ?.reflexivity eq (CM?.mult m (xsdenote eq m am [x]) (xsdenote eq m am xs2)))
+  | x::xs1' ->
+      flatten_correct_aux eq m am xs1' xs2;
+      EQ?.reflexivity eq (select x am);
+      CM?.congruence m (select x am) (xsdenote eq m am (xs1' @ xs2))
+                       (select x am) (CM?.mult m (xsdenote eq m am xs1') (xsdenote eq m am xs2));
+      CM?.associativity m (select x am) (xsdenote eq m am xs1') (xsdenote eq m am xs2);
+      EQ?.symmetry eq (CM?.mult m (CM?.mult m (select x am) (xsdenote eq m am xs1')) (xsdenote eq m am xs2))
+                      (CM?.mult m (select x am) (CM?.mult m (xsdenote eq m am xs1') (xsdenote eq m am xs2)));
+      EQ?.transitivity eq (CM?.mult m (select x am) (xsdenote eq m am (xs1' @ xs2)))
+                          (CM?.mult m (select x am) (CM?.mult m (xsdenote eq m am xs1') (xsdenote eq m am xs2)))
+                          (CM?.mult m (CM?.mult m (select x am) (xsdenote eq m am xs1')) (xsdenote eq m am xs2))
+
+let rec flatten_correct (#a:Type) (eq:equiv a) (m:cm a eq) (am:amap a) (e:exp)
+  : Lemma (mdenote eq m am e `EQ?.eq eq` xsdenote eq m am (flatten e)) =
+  match e with
+  | Unit -> EQ?.reflexivity eq (CM?.unit m)
+  | Atom x -> EQ?.reflexivity eq (select x am)
+  | Mult e1 e2 ->
+      flatten_correct_aux eq m am (flatten e1) (flatten e2);
+      EQ?.symmetry eq (xsdenote eq m am (flatten e1 @ flatten e2))
+                      (CM?.mult m (xsdenote eq m am (flatten e1)) (xsdenote eq m am (flatten e2)));
+      flatten_correct eq m am e1;
+      flatten_correct eq m am e2;
+      CM?.congruence m (mdenote eq m am e1) (mdenote eq m am e2)
+                       (xsdenote eq m am (flatten e1)) (xsdenote eq m am (flatten e2));
+      EQ?.transitivity eq (CM?.mult m (mdenote eq m am e1) (mdenote eq m am e2))
+                          (CM?.mult m (xsdenote eq m am (flatten e1)) (xsdenote eq m am (flatten e2)))
+                          (xsdenote eq m am (flatten e1 @ flatten e2))
+
+let monoid_reflect (#a:Type) (eq:equiv a) (m:cm a eq) (am:amap a) (e1 e2:exp)
+    (_ : squash (xsdenote eq m am (flatten e1) `EQ?.eq eq` xsdenote eq m am (flatten e2)))
+       : squash (mdenote eq m am e1 `EQ?.eq eq` mdenote eq m am e2) =
+    flatten_correct eq m am e1;
+    flatten_correct eq m am e2;
+    EQ?.symmetry eq (mdenote eq m am e2) (xsdenote eq m am (flatten e2));
+    EQ?.transitivity eq
+      (xsdenote eq m am (flatten e1))
+      (xsdenote eq m am (flatten e2))
+      (mdenote eq m am e2);
+    EQ?.transitivity eq
+      (mdenote eq m am e1)
+      (xsdenote eq m am (flatten e1))
+      (mdenote eq m am e2)
+
+// Here we sort the variable numbers
+
+let permute = list atom -> list atom
+let sort : permute = List.Tot.Base.sortWith #int (List.Tot.Base.compare_of_bool (<))
+
+#push-options "--fuel 1 --ifuel 1"
+
+let lemma_xsdenote_aux (#a:Type) (eq:equiv a) (m:cm a eq) (am:amap a) (hd:atom) (tl:list atom)
+  : Lemma (xsdenote eq m am (hd::tl) `EQ?.eq eq`
+         (CM?.mult m (select hd am) (xsdenote eq m am tl)))
+  = match tl with
+    | [] ->
+      assert (xsdenote eq m am (hd::tl) == select hd am);
+      CM?.identity m (select hd am);
+      EQ?.symmetry eq (CM?.unit m `CM?.mult m` select hd am) (select hd am);
+      CM?.commutativity m (CM?.unit m) (select hd am);
+      EQ?.transitivity eq
+        (xsdenote eq m am (hd::tl))
+        (CM?.unit m `CM?.mult m` select hd am)
+        (CM?.mult m (select hd am) (xsdenote eq m am tl))
+    | _ -> EQ?.reflexivity eq (xsdenote eq m am (hd::tl))
+
+let rec partition_equiv (#a:Type) (eq:equiv a) (m:cm a eq) (am:amap a) (pivot:atom) (q:list atom)
+  : Lemma
+    (let open FStar.List.Tot.Base in
+     let hi, lo = partition (bool_of_compare (compare_of_bool (<)) pivot) q in
+     EQ?.eq eq
+      (xsdenote eq m am hi `CM?.mult m` xsdenote eq m am lo)
+      (xsdenote eq m am q))
+   = let open FStar.List.Tot.Base in
+     let f = bool_of_compare (compare_of_bool (<)) pivot in
+     let hi, lo = partition f q in
+     match q with
+     | [] -> CM?.identity m (xsdenote eq m am hi)
+     | hd::tl ->
+         let l1, l2 = partition f tl in
+         partition_equiv eq m am pivot tl;
+         assert (EQ?.eq eq
+           (xsdenote eq m am l1 `CM?.mult m` xsdenote eq m am l2)
+           (xsdenote eq m am tl));
+
+         EQ?.reflexivity eq (xsdenote eq m am l1);
+         EQ?.reflexivity eq (xsdenote eq m am l2);
+         EQ?.reflexivity eq (xsdenote eq m am hi);
+         EQ?.reflexivity eq (xsdenote eq m am lo);
+
+
+         if f hd then begin
+           assert (hi == hd::l1 /\ lo == l2);
+           lemma_xsdenote_aux eq m am hd l1;
+           CM?.congruence m
+             (xsdenote eq m am hi)
+             (xsdenote eq m am lo)
+             (select hd am `CM?.mult m` xsdenote eq m am l1)
+             (xsdenote eq m am l2);
+           CM?.associativity m
+             (select hd am)
+             (xsdenote eq m am l1)
+             (xsdenote eq m am l2);
+           EQ?.transitivity eq
+             (xsdenote eq m am hi `CM?.mult m` xsdenote eq m am lo)
+             ((select hd am `CM?.mult m` xsdenote eq m am l1) `CM?.mult m` xsdenote eq m am l2)
+             (select hd am `CM?.mult m` (xsdenote eq m am l1 `CM?.mult m` xsdenote eq m am l2));
+
+           EQ?.reflexivity eq (select hd am);
+           CM?.congruence m
+             (select hd am)
+             (xsdenote eq m am l1 `CM?.mult m` xsdenote eq m am l2)
+             (select hd am)
+             (xsdenote eq m am tl);
+           EQ?.transitivity eq
+             (xsdenote eq m am hi `CM?.mult m` xsdenote eq m am lo)
+             (select hd am `CM?.mult m` (xsdenote eq m am l1 `CM?.mult m` xsdenote eq m am l2))
+             (select hd am `CM?.mult m` xsdenote eq m am tl);
+
+           lemma_xsdenote_aux eq m am hd tl;
+           EQ?.symmetry eq
+             (xsdenote eq m am (hd::tl))
+             (select hd am `CM?.mult m` xsdenote eq m am tl);
+           EQ?.transitivity eq
+             (xsdenote eq m am hi `CM?.mult m` xsdenote eq m am lo)
+             (select hd am `CM?.mult m` xsdenote eq m am tl)
+             (xsdenote eq m am (hd::tl))
+
+         end else begin
+           assert (hi == l1 /\ lo == hd::l2);
+           lemma_xsdenote_aux eq m am hd l2;
+           CM?.congruence m
+             (xsdenote eq m am hi)
+             (xsdenote eq m am lo)
+             (xsdenote eq m am l1)
+             (select hd am `CM?.mult m` xsdenote eq m am l2);
+           CM?.commutativity m
+             (xsdenote eq m am l1)
+             (select hd am `CM?.mult m` xsdenote eq m am l2);
+           EQ?.transitivity eq
+             (xsdenote eq m am hi `CM?.mult m` xsdenote eq m am lo)
+             (xsdenote eq m am l1 `CM?.mult m` (select hd am `CM?.mult m` xsdenote eq m am l2))
+             ((select hd am `CM?.mult m` xsdenote eq m am l2) `CM?.mult m` xsdenote eq m am l1);
+
+           CM?.associativity m
+             (select hd am)
+             (xsdenote eq m am l2)
+             (xsdenote eq m am l1);
+           EQ?.transitivity eq
+             (xsdenote eq m am hi `CM?.mult m` xsdenote eq m am lo)
+             ((select hd am `CM?.mult m` xsdenote eq m am l2) `CM?.mult m` xsdenote eq m am l1)
+             (select hd am `CM?.mult m` (xsdenote eq m am l2 `CM?.mult m` xsdenote eq m am l1));
+
+           CM?.commutativity m (xsdenote eq m am l2) (xsdenote eq m am l1);
+           EQ?.reflexivity eq (select hd am);
+           CM?.congruence m
+             (select hd am)
+             (xsdenote eq m am l2 `CM?.mult m` xsdenote eq m am l1)
+             (select hd am)
+             (xsdenote eq m am l1 `CM?.mult m` xsdenote eq m am l2);
+           EQ?.transitivity eq
+             (xsdenote eq m am hi `CM?.mult m` xsdenote eq m am lo)
+             (select hd am `CM?.mult m` (xsdenote eq m am l2 `CM?.mult m` xsdenote eq m am l1))
+             (select hd am `CM?.mult m` (xsdenote eq m am l1 `CM?.mult m` xsdenote eq m am l2));
+
+           CM?.congruence m
+             (select hd am)
+             (xsdenote eq m am l1 `CM?.mult m` xsdenote eq m am l2)
+             (select hd am)
+             (xsdenote eq m am tl);
+           EQ?.transitivity eq
+             (xsdenote eq m am hi `CM?.mult m` xsdenote eq m am lo)
+             (select hd am `CM?.mult m` (xsdenote eq m am l1 `CM?.mult m` xsdenote eq m am l2))
+             (select hd am `CM?.mult m` xsdenote eq m am tl);
+
+           lemma_xsdenote_aux eq m am hd tl;
+           EQ?.symmetry eq
+             (xsdenote eq m am (hd::tl))
+             (select hd am `CM?.mult m` xsdenote eq m am tl);
+           EQ?.transitivity eq
+             (xsdenote eq m am hi `CM?.mult m` xsdenote eq m am lo)
+             (select hd am `CM?.mult m` xsdenote eq m am tl)
+             (xsdenote eq m am (hd::tl))
+         end
+
+let rec sort_correct_aux (#a:Type) (eq:equiv a) (m:cm a eq) (am:amap a) (xs:list atom)
+  : Lemma (requires True)
+          (ensures xsdenote eq m am xs `EQ?.eq eq` xsdenote eq m am (sort xs))
+          (decreases (FStar.List.Tot.Base.length xs))
+  = match xs with
+  | [] -> EQ?.reflexivity eq (xsdenote eq m am [])
+  | pivot::q ->
+      let open FStar.List.Tot.Base in
+      let f:int -> int -> int = compare_of_bool (<) in
+      let hi, lo = partition (bool_of_compare f pivot) q in
+      flatten_correct_aux eq m am (sort lo) (pivot::sort hi);
+      assert (xsdenote eq m am (sort xs) `EQ?.eq eq`
+        CM?.mult m (xsdenote eq m am (sort lo))
+                   (xsdenote eq m am (pivot::sort hi)));
+
+      lemma_xsdenote_aux eq m am pivot (sort hi);
+
+      EQ?.reflexivity eq (xsdenote eq m am (sort lo));
+      CM?.congruence m
+        (xsdenote eq m am (sort lo))
+        (xsdenote eq m am (pivot::sort hi))
+        (xsdenote eq m am (sort lo))
+        (select pivot am `CM?.mult m` xsdenote eq m am (sort hi));
+      EQ?.transitivity eq
+        (xsdenote eq m am (sort xs))
+        (xsdenote eq m am (sort lo) `CM?.mult m` xsdenote eq m am (pivot::sort hi))
+        (xsdenote eq m am (sort lo) `CM?.mult m` (select pivot am `CM?.mult m` xsdenote eq m am (sort hi)));
+      assert (EQ?.eq eq
+        (xsdenote eq m am (sort xs))
+        (xsdenote eq m am (sort lo) `CM?.mult m` (select pivot am `CM?.mult m` xsdenote eq m am (sort hi))));
+
+      CM?.commutativity m
+        (xsdenote eq m am (sort lo))
+        (select pivot am `CM?.mult m` xsdenote eq m am (sort hi));
+      CM?.associativity m
+        (select pivot am)
+        (xsdenote eq m am (sort hi))
+        (xsdenote eq m am (sort lo));
+      EQ?.transitivity eq
+         (xsdenote eq m am (sort lo) `CM?.mult m` (select pivot am `CM?.mult m` xsdenote eq m am (sort hi)))
+        ((select pivot am `CM?.mult m` xsdenote eq m am (sort hi)) `CM?.mult m` xsdenote eq m am (sort lo))
+        (select pivot am `CM?.mult m` (xsdenote eq m am (sort hi) `CM?.mult m` xsdenote eq m am (sort lo)));
+      EQ?.transitivity eq
+         (xsdenote eq m am (sort xs))
+         (xsdenote eq m am (sort lo) `CM?.mult m` (select pivot am `CM?.mult m` xsdenote eq m am (sort hi)))
+        (select pivot am `CM?.mult m` (xsdenote eq m am (sort hi) `CM?.mult m` xsdenote eq m am (sort lo)));
+      assert (EQ?.eq eq
+        (xsdenote eq m am (sort xs))
+        (select pivot am `CM?.mult m` (xsdenote eq m am (sort hi) `CM?.mult m` xsdenote eq m am (sort lo))));
+
+
+      partition_length (bool_of_compare f pivot) q;
+      sort_correct_aux eq m am hi;
+      sort_correct_aux eq m am lo;
+      EQ?.symmetry eq (xsdenote eq m am lo) (xsdenote eq m am (sort lo));
+      EQ?.symmetry eq (xsdenote eq m am hi) (xsdenote eq m am (sort hi));
+      CM?.congruence m
+        (xsdenote eq m am (sort hi))
+        (xsdenote eq m am (sort lo))
+        (xsdenote eq m am hi)
+        (xsdenote eq m am lo);
+      assert (EQ?.eq eq
+        (xsdenote eq m am (sort hi) `CM?.mult m` xsdenote eq m am (sort lo))
+        (xsdenote eq m am hi `CM?.mult m` xsdenote eq m am lo));
+
+      EQ?.reflexivity eq (select pivot am);
+      CM?.congruence m
+        (select pivot am)
+        (xsdenote eq m am (sort hi) `CM?.mult m` xsdenote eq m am (sort lo))
+        (select pivot am)
+        (xsdenote eq m am hi `CM?.mult m` xsdenote eq m am lo);
+      EQ?.transitivity eq
+        (xsdenote eq m am (sort xs))
+        (select pivot am `CM?.mult m` (xsdenote eq m am (sort hi) `CM?.mult m` xsdenote eq m am (sort lo)))
+        (select pivot am `CM?.mult m` (xsdenote eq m am hi `CM?.mult m` xsdenote eq m am lo));
+      assert (EQ?.eq eq
+        (xsdenote eq m am (sort xs))
+        (select pivot am `CM?.mult m` (xsdenote eq m am hi `CM?.mult m` xsdenote eq m am lo)));
+
+      partition_equiv eq m am pivot q;
+      CM?.congruence m
+        (select pivot am)
+        (xsdenote eq m am hi `CM?.mult m` xsdenote eq m am lo)
+        (select pivot am)
+        (xsdenote eq m am q);
+      EQ?.transitivity eq
+        (xsdenote eq m am (sort xs))
+        (select pivot am `CM?.mult m` (xsdenote eq m am hi `CM?.mult m` xsdenote eq m am lo))
+        (select pivot am `CM?.mult m` (xsdenote eq m am q));
+      assert (EQ?.eq eq
+        (xsdenote eq m am (sort xs))
+        (select pivot am `CM?.mult m` (xsdenote eq m am q)));
+
+      lemma_xsdenote_aux eq m am pivot q;
+      EQ?.symmetry eq
+        (xsdenote eq m am (pivot::q))
+        (select pivot am `CM?.mult m` (xsdenote eq m am q));
+      EQ?.transitivity eq
+        (xsdenote eq m am (sort xs))
+        (select pivot am `CM?.mult m` (xsdenote eq m am q))
+        (xsdenote eq m am xs);
+      EQ?.symmetry eq (xsdenote eq m am (sort xs)) (xsdenote eq m am xs)
+
+#pop-options
+
+#push-options "--fuel 0 --ifuel 0"
+
+let identity_left (#a:Type) (eq:equiv a) (m:cm a eq) (x:a)
+  : Lemma (EQ?.eq eq x (CM?.mult m (CM?.unit m) x))
+  = CM?.identity m x;
+    EQ?.symmetry eq (CM?.mult m (CM?.unit m) x) x
+
+let identity_right_diff (#a:Type) (eq:equiv a) (m:cm a eq) (x y:a) : Lemma
+  (requires EQ?.eq eq x y)
+  (ensures EQ?.eq eq (CM?.mult m x (CM?.unit m)) y)
+  = right_identity eq m x;
+    EQ?.transitivity eq (CM?.mult m x (CM?.unit m)) x y
+
+let rec dismiss_slprops () : Tac unit =
+  match term_as_formula' (cur_goal ()) with
+    | App t _ -> if term_eq t (`squash) then () else (dismiss(); dismiss_slprops ())
+    | _ -> dismiss(); dismiss_slprops ()
+
+let rec n_identity_left (n:int) (eq m:term) : Tac unit
+  = if n = 0 then (
+      apply_lemma (`(EQ?.reflexivity (`#eq)));
+      // Cleaning up, in case a uvar has been generated here. It'll be solved later
+      set_goals [])
+    else (
+      apply_lemma (`identity_right_diff (`#eq) (`#m));
+      // Drop the slprops generated, they will be solved later
+      dismiss_slprops ();
+      n_identity_left (n-1) eq m
+    )
+
+let equivalent_sorted (#a:Type) (eq:equiv a) (m:cm a eq) (am:amap a) (l1 l2 l1' l2':list atom)
+    : Lemma (requires
+              sort l1 == sort l1' /\
+              sort l2 == sort l2' /\
+              xsdenote eq m am l1 `EQ?.eq eq` xsdenote eq m am l2)
+           (ensures xsdenote eq m am l1' `EQ?.eq eq` xsdenote eq m am l2')
+  = sort_correct_aux eq m am l1';
+    sort_correct_aux eq m am l1;
+    EQ?.symmetry eq (xsdenote eq m am l1) (xsdenote eq m am (sort l1));
+    EQ?.transitivity eq
+      (xsdenote eq m am l1')
+      (xsdenote eq m am (sort l1'))
+      (xsdenote eq m am l1);
+    EQ?.transitivity eq
+      (xsdenote eq m am l1')
+      (xsdenote eq m am l1)
+      (xsdenote eq m am l2);
+    sort_correct_aux eq m am l2;
+    EQ?.transitivity eq
+      (xsdenote eq m am l1')
+      (xsdenote eq m am l2)
+      (xsdenote eq m am (sort l2));
+    sort_correct_aux eq m am l2';
+    EQ?.symmetry eq (xsdenote eq m am l2') (xsdenote eq m am (sort l2'));
+    EQ?.transitivity eq
+      (xsdenote eq m am l1')
+      (xsdenote eq m am (sort l2))
+      (xsdenote eq m am l2')
+
+#pop-options
+
+(* Finds the position of first occurrence of x in xs.
+   This is now specialized to terms and their funny term_eq. *)
+let rec where_aux (n:nat) (x:term) (xs:list term) :
+    Tot (option nat) (decreases xs) =
+  match xs with
+  | [] -> None
+  | x'::xs' -> if term_eq x x' then Some n else where_aux (n+1) x xs'
+let where = where_aux 0
+
+let fatom (t:term) (ts:list term) (am:amap term) : Tac (exp * list term * amap term) =
+  match where t ts with
+  | Some v -> (Atom v, ts, am)
+  | None ->
+    let vfresh = List.Tot.Base.length ts in
+    let t = norm_term [iota; zeta] t in
+    (Atom vfresh, ts @ [t], update vfresh t am)
+
+// This expects that mult, unit, and t have already been normalized
+let rec reification_aux (ts:list term) (am:amap term)
+                        (mult unit t : term) : Tac (exp * list term * amap term) =
+  let hd, tl = collect_app_ref t in
+  match inspect hd, List.Tot.Base.list_unref tl with
+  | Tv_FVar fv, [(t1, Q_Explicit) ; (t2, Q_Explicit)] ->
+    if term_eq (pack (Tv_FVar fv)) mult
+    then (let (e1, ts, am) = reification_aux ts am mult unit t1 in
+          let (e2, ts, am) = reification_aux ts am mult unit t2 in
+          (Mult e1 e2, ts, am))
+    else fatom t ts am
+  | _, _ ->
+    if term_eq t unit
+    then (Unit, ts, am)
+    else fatom t ts am
+
+let reification (eq: term) (m: term) (ts:list term) (am:amap term) (t:term) :
+    Tac (exp * list term * amap term) =
+  let mult = norm_term [iota; zeta; delta] (`CM?.mult (`#m)) in
+  let unit = norm_term [iota; zeta; delta] (`CM?.unit (`#m)) in
+  let t    = norm_term [iota; zeta] t in
+  reification_aux ts am mult unit t
+
+let rec convert_map (m : list (atom * term)) : term =
+  match m with
+  | [] -> `[]
+  | (a, t)::ps ->
+      let a = pack_ln (Tv_Const (C_Int a)) in
+      (* let t = norm_term [delta] t in *)
+      `((`#a, (`#t)) :: (`#(convert_map ps)))
+
+
+(* `am` is an amap (basically a list) of terms, each representing a value
+of type `a` (whichever we are canonicalizing). This functions converts
+`am` into a single `term` of type `amap a`, suitable to call `mdenote` with *)
+let convert_am (am : amap term) : term =
+  let (map, def) = am in
+  (* let def = norm_term [delta] def in *)
+  `( (`#(convert_map map), `#def) )
+
+let rec quote_exp (e:exp) : term =
+    match e with
+    | Unit -> (`Unit)
+    | Mult e1 e2 -> (`Mult (`#(quote_exp e1)) (`#(quote_exp e2)))
+    | Atom n -> let nt = pack_ln (Tv_Const (C_Int n)) in
+                (`Atom (`#nt))
+
+let rec quote_atoms (l:list atom) = match l with
+  | [] -> `[]
+  | hd::tl -> let nt = pack_ln (Tv_Const (C_Int hd)) in
+              (`Cons (`#nt) (`#(quote_atoms tl)))
+
+let normal_steps = [primops; iota; zeta; delta_only [
+          `%mdenote; `%select; `%List.Tot.Base.assoc; `%List.Tot.Base.append;
+          `%flatten; `%sort;
+          `%List.Tot.Base.sortWith; `%List.Tot.Base.partition;
+          `%List.Tot.Base.bool_of_compare; `%List.Tot.Base.compare_of_bool;
+          `%fst; `%__proj__Mktuple2__item___1;
+          `%snd; `%__proj__Mktuple2__item___2;
+          `%__proj__CM__item__unit;
+          `%__proj__CM__item__mult;
+          `%rm]]
+
+let normal_tac (#a:Type) (x:a) : a = FStar.Pervasives.norm normal_steps x
+
+let normal_elim (x:Type0) : Lemma
+  (requires x)
+  (ensures normal_tac x)
+  = ()
+
+let canon_l_r (eq: term) (m: term) (lhs rhs:term) : Tac unit =
+  let m_unit = norm_term [iota; zeta; delta](`CM?.unit (`#m)) in
+  let am = const m_unit in (* empty map *)
+  let (r1_raw, ts, am) = reification eq m [] am lhs in
+  let (r2_raw,  _, am) = reification eq m ts am rhs in
+
+  let l1_raw, l2_raw, emp_frame = equivalent_lists (flatten r1_raw) (flatten r2_raw) am in
+
+  let am = convert_am am in
+  let r1 = quote_exp r1_raw in
+  let r2 = quote_exp r2_raw in
+  let l1 = quote_atoms l1_raw in
+  let l2 = quote_atoms l2_raw in
+  change_sq (`(normal_tac (mdenote (`#eq) (`#m) (`#am) (`#r1)
+                 `EQ?.eq (`#eq)`
+               mdenote (`#eq) (`#m) (`#am) (`#r2))));
+  apply_lemma (`normal_elim);
+
+  apply (`monoid_reflect );
+
+
+  apply_lemma (`equivalent_sorted (`#eq) (`#m) (`#am) (`#l1) (`#l2));
+  let g = goals () in
+  if List.Tot.Base.length g = 0 then
+    // The application of equivalent_sorted seems to sometimes solve
+    // all goals
+    ()
+  else (
+    norm [primops; iota; zeta; delta_only
+      [`%xsdenote; `%select; `%List.Tot.Base.assoc; `%List.Tot.Base.append;
+        `%flatten; `%sort;
+        `%List.Tot.Base.sortWith; `%List.Tot.Base.partition;
+        `%List.Tot.Base.bool_of_compare; `%List.Tot.Base.compare_of_bool;
+        `%fst; `%__proj__Mktuple2__item___1;
+        `%snd; `%__proj__Mktuple2__item___2;
+        `%__proj__CM__item__unit;
+        `%__proj__CM__item__mult;
+        `%rm
+
+        ]];
+
+    split();
+    split();
+    // equivalent_lists should have built valid permutations.
+    // If that's not the case, it is a bug in equivalent_lists
+    or_else trefl (fun _ -> fail "first equivalent_lists did not build a valid permutation");
+    or_else trefl (fun _ -> fail "second equivalent_lists did not build a valid permutation");
+
+    if emp_frame then apply_lemma (`identity_left (`#eq) (`#m))
+    else apply_lemma (`(EQ?.reflexivity (`#eq)))
+  )
+
+
+let canon_monoid (eq:term) (m:term) : Tac unit =
+  norm [iota; zeta];
+  let t = cur_goal () in
+  // removing top-level squash application
+  let sq, rel_xy = collect_app_ref t in
+  // unpacking the application of the equivalence relation (lhs `EQ?.eq eq` rhs)
+  (match rel_xy with
+   | [(rel_xy,_)] -> (
+       let open FStar.List.Tot.Base in
+       let rel, xy = collect_app_ref rel_xy in
+       if (length xy >= 2)
+       then (
+         match index xy (length xy - 2) , index xy (length xy - 1) with
+         | (lhs, Q_Explicit) , (rhs, Q_Explicit) ->
+           canon_l_r eq m lhs rhs
+         | _ -> fail "Goal should have been an application of a binary relation to 2 explicit arguments"
+       )
+       else (
+         fail "Goal should have been an application of a binary relation to n implicit and 2 explicit arguments"
+       )
+     )
+   | _ -> fail "Goal should be squash applied to a binary relation")
+
+(* Try to integrate it into larger tactic *)
+
+let canon' () : Tac unit =
+  canon_monoid (`req) (`rm)
+
+(* A Variant of canon to collect all slprops in the context into the return_post term,
+   and set all extra uvars to emp *)
+
+let rec slterm_nbr_uvars (t:term) : Tac int =
+  match inspect t with
+  | Tv_Uvar _ _ -> 1
+  | Tv_App _ _ ->
+    let hd, args = collect_app t in
+    if term_eq hd (`star) then
+
+      // Only count the number of unresolved slprops, not program implicits
+      fold_left (fun n (x, _) -> n + slterm_nbr_uvars x) 0 args
+    else if is_uvar hd then 1
+    else 0
+  | Tv_Abs _ t -> slterm_nbr_uvars t
+  | _ -> 0
+
+
+/// Puts the term containing return_post at the top.
+/// Returns the atom corresponding to return_post, and the list with the atom removed
+let rec return_at_top' (l:list atom) (am:amap term) : Tac (atom * list atom) =
+  match l with
+  | [] -> fail "Couldn't find return_post term"
+  | hd::tl ->
+      if term_appears_in (`return_post) (select hd am) then hd, tl else
+      let ret, rest = return_at_top' tl am in
+      ret, hd::rest
+
+/// Checks whether the return slprop is fully resolved
+let return_resolved (l:list atom) (am:amap term) : Tac bool =
+  let ret, _ = return_at_top' l am in
+  let t = norm_term [delta_only [`%return_post]] (select ret am) in
+  slterm_nbr_uvars t = 0
+
+let return_at_top (l:list atom) (am:amap term) : Tac (nat * list atom) =
+  let ret, tl = return_at_top' l am in
+  List.Tot.Base.length tl, ret :: tl
+
+exception AlreadyGathered
+
+let gather_return (eq: term) (m: term) (lhs rhs:term) : Tac unit =
+  let return_lhs = term_appears_in (`return_post) lhs in
+  let return_rhs = term_appears_in (`return_post) rhs in
+  let two_returns = return_lhs && return_rhs in
+
+  let lhs, rhs =
+    // Ensure that the return_post is on the left
+    if return_rhs && not (return_lhs) then
+      (apply_lemma (`equiv_sym); rhs, lhs) else lhs, rhs
+  in
+
+
+  let m_unit = norm_term [iota; zeta; delta](`CM?.unit (`#m)) in
+  let am = const m_unit in (* empty map *)
+  let (r1_raw, ts, am) = reification eq m [] am lhs in
+  let (r2_raw,  _, am) = reification eq m ts am rhs in
+
+  let l1_raw = flatten r1_raw in
+  let l2_raw = flatten r2_raw in
+
+  let resolved1 = return_resolved l1_raw am in
+  let resolved2 = if two_returns then return_resolved l2_raw am else true in
+
+  if resolved1 && resolved2 then (
+    // The return_post have already been gathered, we will fall back on the normal canon
+    raise AlreadyGathered
+  ) else (
+
+    let n_l1, l1_raw = return_at_top l1_raw am in
+
+    let n_l2, l2_raw = if two_returns then return_at_top l2_raw am else 0, l2_raw in
+
+    let am = convert_am am in
+    let r1 = quote_exp r1_raw in
+    let r2 = quote_exp r2_raw in
+    change_sq (`(normal (mdenote (`#eq) (`#m) (`#am) (`#r1)
+                   `EQ?.eq (`#eq)`
+                 mdenote (`#eq) (`#m) (`#am) (`#r2))));
+    apply_lemma (`normal_elim);
+
+    apply (`monoid_reflect );
+
+    let l1 = quote_atoms l1_raw in
+    let l2 = quote_atoms l2_raw in
+
+    apply_lemma (`equivalent_sorted (`#eq) (`#m) (`#am) (`#l1) (`#l2));
+    let g = goals () in
+    if List.Tot.Base.length g = 0 then
+      // The application of equivalent_sorted seems to sometimes solve
+      // all goals
+      ()
+    else (
+      norm [primops; iota; zeta; delta_only
+        [`%xsdenote; `%select; `%List.Tot.Base.assoc; `%List.Tot.Base.append;
+          `%flatten; `%sort;
+          `%return_post;
+          `%List.Tot.Base.sortWith; `%List.Tot.Base.partition;
+          `%List.Tot.Base.bool_of_compare; `%List.Tot.Base.compare_of_bool;
+          `%fst; `%__proj__Mktuple2__item___1;
+          `%snd; `%__proj__Mktuple2__item___2;
+          `%__proj__CM__item__unit;
+          `%__proj__CM__item__mult;
+          `%rm
+
+          ]];
+
+      split();
+      split();
+      // equivalent_lists should have built valid permutations.
+      // If that's not the case, it is a bug in equivalent_lists
+      or_else trefl (fun _ -> fail "first equivalent_lists did not build a valid permutation");
+      or_else trefl (fun _ -> fail "second equivalent_lists did not build a valid permutation");
+
+      if n_l2 > n_l1 then
+        (apply_lemma (`(EQ?.symmetry (`#eq)));
+         dismiss_slprops();
+         let n = n_l2 - n_l1 in
+         focus (fun _ -> n_identity_left n eq m))
+      else (let n = n_l1 - n_l2 in focus (fun _ -> n_identity_left n eq m))
+    )
+  )
+
+let canon_return' (eq:term) (m:term) : Tac unit =
+  norm [iota; zeta];
+  let t = cur_goal () in
+  // removing top-level squash application
+  let sq, rel_xy = collect_app_ref t in
+  // unpacking the application of the equivalence relation (lhs `EQ?.eq eq` rhs)
+  (match rel_xy with
+   | [(rel_xy,_)] -> (
+       let open FStar.List.Tot.Base in
+       let rel, xy = collect_app_ref rel_xy in
+       if (length xy >= 2)
+       then (
+         match index xy (length xy - 2) , index xy (length xy - 1) with
+         | (lhs, Q_Explicit) , (rhs, Q_Explicit) ->
+           gather_return eq m lhs rhs
+         | _ -> fail "Goal should have been an application of a binary relation to 2 explicit arguments"
+       )
+       else (
+         fail "Goal should have been an application of a binary relation to n implicit and 2 explicit arguments"
+       )
+     )
+   | _ -> fail "Goal should be squash applied to a binary relation")
+
+let canon_return () : Tac unit =
+  canon_return' (`req) (`rm)
+
+
+
+
+let typ_contains_req_ens (t:term) : Tac bool =
+  let name, _ = collect_app t in
+  if term_eq name (`req_t) || term_eq name (`ens_t) then true
+  else false
+
+let rec filter_goals (l:list goal) : Tac (list goal * list goal) =
+  match l with
+  | [] -> [], []
+  | hd::tl ->
+      let slgoals, loggoals = filter_goals tl in
+      match term_as_formula' (goal_type hd) with
+      | Comp (Eq t) _ _ ->
+        if Some? t then
+          let b = typ_contains_req_ens (Some?.v t) in
+          if b then slgoals, hd::loggoals
+          else hd::slgoals, loggoals
+        else hd::slgoals, loggoals
+      | App t _ -> if term_eq t (`squash) then hd::slgoals, loggoals else slgoals, loggoals
+      | _ -> slgoals, loggoals
+
+let is_return_eq (l r:term) : Tac bool =
+  let nl, al = collect_app l in
+  let nr, ar = collect_app r in
+  term_eq nl (`return_pre) || term_eq nr (`return_pre)
+
+let rec solve_indirection_eqs (l:list goal) : Tac unit =
+  match l with
+  | [] -> ()
+  | hd::tl ->
+    let f = term_as_formula' (goal_type hd) in
+    match f with
+    | Comp (Eq _) l r ->
+        if is_return_eq l r then later() else trefl();
+        solve_indirection_eqs tl
+    | _ -> later(); solve_indirection_eqs tl
+
+
+let rec solve_return_eqs (l:list goal) : Tac unit =
+  match l with
+  | [] -> ()
+  | hd::tl ->
+    let f = term_as_formula' (goal_type hd) in
+    match f with
+    | Comp (Eq _) l r ->
+        trefl();
+        solve_return_eqs tl
+    | _ -> later(); solve_return_eqs tl
+
+// The term corresponds to a goal containing a return_post
+let solve_return (t:term) : Tac unit
+  = dump "entering return";
+    // Remove potential annotations first
+    if term_appears_in (`can_be_split) t then (
+      apply_lemma (`equiv_can_be_split)
+    ) else if term_appears_in (`can_be_split_forall) t then (
+      ignore (forall_intro ());
+      apply_lemma (`equiv_can_be_split)
+    ) else if term_appears_in (`equiv_forall) t then (
+      fail "equiv_forall"
+      // apply_lemma (`equiv_forall_elim);
+      // ignore (forall_intro())
+    ) else if term_appears_in (`can_be_split_post) t then (
+      fail "can_be_split_post"
+      // apply_lemma (`can_be_split_post_elim);
+      // dismiss_slprops();
+      // ignore (forall_intro ());
+      // ignore (forall_intro ())
+    ) else
+      // This should never happen
+      fail "return_post goal in unexpected position";
+    match (goals ()) with
+    | [] -> () // Can happen if reflexivity was sufficient here
+    | _ -> norm [delta_only [
+                     `%CE.__proj__CM__item__unit;
+                     `%CE.__proj__CM__item__mult;
+                     `%rm;
+                     `%__proj__Mktuple2__item___1; `%__proj__Mktuple2__item___2;
+                     `%fst; `%snd];
+//               delta_attr [`%__reduce__];
+               primops; iota; zeta];
+           canon_return ()
+
+
+let rec solve_all_returns (l:list goal) : Tac unit =
+  match l with
+  | [] -> ()
+  | hd::tl ->
+    let t = goal_type hd in
+    let f = term_as_formula' t in
+    dump "entering solve";
+    if term_appears_in (`return_post) t then (
+      try focus (fun _ -> solve_return t) with
+        // If return_post has already been gathered, we remove the annotation, and will solve this constraint normally later
+        | AlreadyGathered -> norm [delta_only [`%return_post]]; later()
+        | TacticFailure m -> fail m
+        | _ -> () // Success
+    ) else later();
+    solve_all_returns tl
+
+
+
+[@@ resolve_implicits; framing_implicit]
+let init_resolve_tac () : Tac unit =
+  // We split goals between framing goals, about slprops (slgs)
+  // and goals related to requires/ensures, that depend on slprops (loggs)
+  let slgs, loggs = filter_goals (goals()) in
+
+  // We first solve the slprops
+  set_goals slgs;
+
+  // We first solve all indirection equalities that will not lead to imprecise unification
+  // i.e. we can solve all equalities inserted by layered effects, except the ones corresponding
+  // to the preconditions of a pure return
+  solve_indirection_eqs (goals());
+
+  // To debug, it is best to look at the goals at this stage. Uncomment the next line
+  // dump "initial goals";
+
+  // We now solve all postconditions of pure returns to avoid restricting the uvars
+  solve_all_returns (goals ());
+
+
+  fail "all"
+
 (* Some tests *)
 
 let test (r:ref int) : SteelSel unit
@@ -359,43 +1695,43 @@ let test (r:ref int) : SteelSel unit
   = write r 1;
     write r 0
 
-let test2 (r1 r2:ref int) : SteelSel unit
-  (vptr r1 `star` vptr r2) (fun _ -> vptr r1 `star` vptr r2)
-  (requires fun _ -> True)
-  (ensures fun h0 _ h1 -> sel h1 r1 == 0 /\ sel h0 r2 == sel h1 r2)
-  = frame (fun _ -> write r1 1) (vptr r2);
-    frame (fun _ -> write r1 0) (vptr r2)
+// let test2 (r1 r2:ref int) : SteelSel unit
+//   (vptr r1 `star` vptr r2) (fun _ -> vptr r1 `star` vptr r2)
+//   (requires fun _ -> True)
+//   (ensures fun h0 _ h1 -> sel h1 r1 == 0 /\ sel h0 r2 == sel h1 r2)
+//   = frame (fun _ -> write r1 1) (vptr r2);
+//     frame (fun _ -> write r1 0) (vptr r2)
 
-// AF: Should work with r3 if we specify the additional can_be_split
-let test3 (r1 r2 r3:ref int) : SteelSel unit
-  (vptr r1 `star` (vptr r2 `star` vptr r3)) (fun _ -> vptr r1 `star` (vptr r2 `star` vptr r3))
-  (requires fun _ ->
-    can_be_split (vptr r1 `star` vptr r2 `star` vptr r3) (vptr r1) /\
-    can_be_split (vptr r1 `star` (vptr r2 `star` vptr r3)) (vptr r2))
-  (ensures fun h0 _ h1 ->
-    can_be_split (vptr r1 `star` vptr r2 `star` vptr r3) (vptr r1) /\
-    can_be_split (vptr r1 `star` (vptr r2 `star` vptr r3)) (vptr r2) /\
-    sel h1 r1 == 0 /\
-    sel h0 r2 == sel h1 r2
-  )
-  = let h0 = get () in
-    frame (fun _ -> write r1 1) (vptr r2 `star` vptr r3);
-    let h1 = get() in
-    assert (sel h1 r1 == 1);
-    assert (sel h0 r2 == sel h1 r2);
-    frame (fun _ -> write r1 0) (vptr r2 `star` vptr r3)
+// // AF: Should work with r3 if we specify the additional can_be_split
+// let test3 (r1 r2 r3:ref int) : SteelSel unit
+//   (vptr r1 `star` (vptr r2 `star` vptr r3)) (fun _ -> vptr r1 `star` (vptr r2 `star` vptr r3))
+//   (requires fun _ ->
+//     can_be_split (vptr r1 `star` vptr r2 `star` vptr r3) (vptr r1) /\
+//     can_be_split (vptr r1 `star` (vptr r2 `star` vptr r3)) (vptr r2))
+//   (ensures fun h0 _ h1 ->
+//     can_be_split (vptr r1 `star` vptr r2 `star` vptr r3) (vptr r1) /\
+//     can_be_split (vptr r1 `star` (vptr r2 `star` vptr r3)) (vptr r2) /\
+//     sel h1 r1 == 0 /\
+//     sel h0 r2 == sel h1 r2
+//   )
+//   = let h0 = get () in
+//     frame (fun _ -> write r1 1) (vptr r2 `star` vptr r3);
+//     let h1 = get() in
+//     assert (sel h1 r1 == 1);
+//     assert (sel h0 r2 == sel h1 r2);
+//     frame (fun _ -> write r1 0) (vptr r2 `star` vptr r3)
 
 
-let swap (#a:Type0) (r1 r2:ref a) : SteelSel unit
-  (vptr r1 `star` vptr r2)
-  (fun _ -> vptr r1 `star` vptr r2)
-  (requires fun _ -> True)
-  (ensures fun h0 _ h1 ->
-    sel h0 r1 == sel h1 r2 /\
-    sel h0 r2 == sel h1 r1)
-  = let x1 = frame (fun _ -> read r1) (vptr r2) in
-    rewrite_2 (vptr r1) (vptr r2);
-    let x2 = frame (fun _ -> read r2) (vptr r1) in
-    frame (fun _ -> write r2 x1) (vptr r1);
-    rewrite_2 (vptr r2) (vptr r1);
-    frame (fun _ -> write r1 x2) (vptr r2)
+// let swap (#a:Type0) (r1 r2:ref a) : SteelSel unit
+//   (vptr r1 `star` vptr r2)
+//   (fun _ -> vptr r1 `star` vptr r2)
+//   (requires fun _ -> True)
+//   (ensures fun h0 _ h1 ->
+//     sel h0 r1 == sel h1 r2 /\
+//     sel h0 r2 == sel h1 r1)
+//   = let x1 = frame (fun _ -> read r1) (vptr r2) in
+//     rewrite_2 (vptr r1) (vptr r2);
+//     let x2 = frame (fun _ -> read r2) (vptr r1) in
+//     frame (fun _ -> write r2 x1) (vptr r1);
+//     rewrite_2 (vptr r2) (vptr r1);
+//     frame (fun _ -> write r1 x2) (vptr r2)
